
$
\left(\int_{-\infty}^{\infty} e^{-x^2}\right) =\int_{-\infty}^{\infty}\int_{-\infty}^{\infty}e^{-(x^2+y^2)}dx \, dy 
`$$

$$`
	 \fbox{$\displaystyle\int_0^\infty f(x)\,{\rm d}x 
	\approx\sum_{i=1}^nw_i{\rm e}^{x_i}f(x_i)$} 
`$$


\[ \left(\int_{-\infty}ˆ{\infty} eˆ{-xˆ2}\right) =\int_{-\infty}ˆ{\infty}\int_{-\infty}ˆ{\infty}eˆ{-(xˆ2+yˆ2)}dx\,dy \]


\begin{displaymath}
\left(\int_{-\infty}ˆ{\infty} eˆ{-xˆ2}\right) =\int_{-\infty}ˆ{\infty}\int_{-\infty}ˆ{\infty}eˆ{-(xˆ2+yˆ2)}dx\,dy 
\end{displaymath}

