
1

$$
\left(\int_{-\infty}^{\infty} e^{-x^2}\right) =\int_{-\infty}^{\infty}\int_{-\infty}^{\infty}e^{-(x^2+y^2)}dx\,dy
 $$

 2
 
$$ 
\left(\int_{-\infty}^{\infty} e^{-x^2}\right) = \int_{-\infty}^{\infty}\int_{-\infty}^{\infty}e^{-(x^2+y^2)}dx\,dy
$$

3


$$
\left(\int_{-\infty}^{\infty} e^{-x^2}\right) = \int_{-\infty}^{\infty}\int_{-\infty}^{\infty}e^{-(x^2+y^2)}dx\,dy
$$

4


$$ 
\left(\int_{-\infty}^{\infty} e^{-x^2}\right) = \int_{-\infty}^{\infty}\int_{-\infty}^{\infty}e^{-(x^2+y^2)}dx\,dy
$$

5

$$
\left(\int_{-\infty}^{\infty} e^{-x^2}\right) = \int_{-\infty}^{\infty}\int_{-\infty}^{\infty}e^{-(x^2+y^2)}dx\,dy
$$
